

# Math Notes



Canine-Table

Github

POSIX Nexus serves as a comprehensive cross-language reference hub that explores the implementation and behavior of POSIX-compliant functionality across a diverse set of programming environments. Built atop the foundational IEEE Portable Operating System Interface (POSIX) standards, this project emphasizes compatibility, portability, and interoperability between operating systems.

## Abstract

## Contents

<b>I</b>	<b>Algebra</b>	<b>II</b>
I	Nomials . . . . .	II
I	Polynomial Exponents . . . . .	IV
I	Dividing Polynomials . . . . .	IX
I	Multiplying Polynomials . . . . .	XI
I	Combining Polynomials . . . . .	XIII
I	FOIL Method . . . . .	XVII
I	Factoring Polynomials . . . . .	XIX
<b>II</b>	<b>Glossary</b>	<b>XXIV</b>



# I Algebra

## I Nomials

### Nomial Lineage

- ➔ **Monomial**  $\Rightarrow$  One term only, e.g.  $7x^2$
- ➔ **Binomial**  $\Rightarrow$  Two terms, e.g.  $x + 2$
- ➔ **Trinomial**  $\Rightarrow$  Three terms, e.g.  $x^2 + 3x + 2$
- ➔ **Polynomial**  $\Rightarrow$  Many terms, general family
- ➔ **Technique**  $\Rightarrow$  Prefix indicates number of terms
- ➔ **Outcome**  $\Rightarrow$  Classification helps organize algebraic expressions

$$\text{Monomial: } ax^n \quad (1)$$

$$\text{Binomial: } ax^n + bx^m \quad (2)$$

$$\text{Trinomial: } ax^n + bx^m + cx^k \quad (3)$$





## Polynomial Forms

- ➔ **Monomial**  $\Rightarrow$  One term only, e.g.  $7x^2$
- ➔ **Binomial**  $\Rightarrow$  Two unlike terms, e.g.  $x + 2$
- ➔ **Trinomial**  $\Rightarrow$  Three terms, e.g.  $x^2 + 3x + 2$
- ➔ **Polynomial**  $\Rightarrow$  General family with many terms
- ➔ **Technique**  $\Rightarrow$  Prefix indicates number of terms
- ➔ **Outcome**  $\Rightarrow$  Classification helps organize algebraic expressions

## Like Terms

- ➔ **Definition**  $\Rightarrow$  Expressions with identical variable parts, e.g.  $3x^2$  and  $-5x^2$
- ➔ **Variable Match**  $\Rightarrow$  Same variables with same exponents
- ➔ **Coefficient**  $\Rightarrow$  Numbers in front may differ
- ➔ **Technique**  $\Rightarrow$  Combine by adding or subtracting coefficients
- ➔ **Outcome**  $\Rightarrow$  Simplifies polynomials by reducing to fewer terms





## Coefficient

- ➔ **Definition**  $\Rightarrow$  The number in front of a variable, e.g. in  $7x$  the coefficient is 7
- ➔ **Variable Match**  $\Rightarrow$  It scales the variable part without changing its type
- ➔ **Examples**  $\Rightarrow 3x^2$  has coefficient 3,  $-5y$  has coefficient -5
- ➔ **Constants**  $\Rightarrow$  A constant term like 4 can be seen as coefficient 4 of  $x^0$
- ➔ **Outcome**  $\Rightarrow$  Coefficients tell how strongly each variable contributes to the polynomial

## I Polynomial Exponents

### Exponent Flip Examples

$$x^5 = \frac{1}{x^{-5}}$$

$$x^{12} = \frac{1}{x^{-12}} \quad (4)$$

$$x^{17} = \frac{1}{x^{-17}}$$

$$15x^9 = \frac{15}{x^{-9}} \quad (5)$$

$$28x^5 = \frac{28}{x^{-5}}$$

$$x^5 = \frac{1}{x^{-5}} \quad (6)$$

$$x^{-3} = \frac{1}{x^3}$$

$$x^3 = \frac{1}{x^{-3}} \quad (7)$$

$$x^{-3} = \frac{1}{x^3}$$

$$(8)$$





$$\begin{aligned}
 (((x^{32y^{5z^3}})^8)^3)^{-9} &= (x^{32y^{5z^3}})^{8 \cdot 3} \Rightarrow x^{768y^{5z^3}} \\
 &= (x^{768y^{5z^3}})^{-9} \Rightarrow x^{-9 \cdot 768y^{5z^3}} \\
 &= x^{-6912y^{5z^3}}
 \end{aligned}$$

### Polynomial Exponent Rules Applied

- ➔ **Power of a Power**  $\Rightarrow (a^m)^n = a^{mn}$
- ➔ **Nested Powers**  $\Rightarrow$  Combine:  $8 \cdot 3 = 24$
- ➔ **Outer Flip**  $\Rightarrow$  Apply  $(-9)$ :  $x^{768y^{5z^3}} \rightarrow x^{-6912y^{5z^3}}$
- ➔ **Technique**  $\Rightarrow$  Multiply all exponents carefully, preserve inner structure
- ➔ **Outcome**  $\Rightarrow$  Final simplified form:  $x^{-6912y^{5z^3}}$

$$\begin{aligned}
 (((x^{32y^{5z^3}})^8)^3)^{-9} &= (x^{32y^{5z^3}})^{8 \cdot 3} \Rightarrow x^{768y^{5z^3}} \\
 &= (x^{768y^{5z^3}})^{-9} \Rightarrow x^{-9 \cdot 768y^{5z^3}} \\
 &= x^{-6912y^{5z^3}}
 \end{aligned}$$



**Exponent Rules Applied**

- ➔ **Power of a Power**  $\Rightarrow (a^m)^n = a^{mn}$
- ➔ **Nested Powers**  $\Rightarrow$  Combine:  $8 \cdot 3 = 24$
- ➔ **Outer Flip**  $\Rightarrow$  Apply  $(-9)$ :  $x^{768}y^{5z^3} \rightarrow x^{-6912}y^{5z^3}$
- ➔ **Technique**  $\Rightarrow$  Multiply all exponents carefully, preserve inner structure
- ➔ **Outcome**  $\Rightarrow$  Final simplified form:  $x^{-6912}y^{5z^3}$

$$x^2 \cdot x^4 = x^{2+4} \Rightarrow x^6$$

$$x^7 \cdot x^5 = x^{5+7} \Rightarrow x^{12}$$

$$x^8 \cdot x^9 = x^{8+9} \Rightarrow x^{17}$$

$$(3x^3)(5x^6) = (3 \cdot 5)x^{3+6} \Rightarrow 15x^9$$

$$(4x^2)(7x^3) = (4 \cdot 7)x^{2+3} \Rightarrow 28x^5$$

$$(4xy^2)(8x^2y^3) = (4 \cdot 8)x^{1+2}(1 \cdot 1)y^{2+3} \Rightarrow 32x^3y^5$$

$$(5x^2y^3)(6x^3y^4) = (5 \cdot 6)x^{2+3}(1 \cdot 1)y^{3+4} \Rightarrow 30x^5y^7$$

$$(7x^3y^4)(8x^5y^7) = (7 \cdot 8)x^{3+5}(1 \cdot 1)y^{4+7} \Rightarrow 56x^8y^{11}$$





$$\begin{aligned}(x^3)^4 &= x^{3 \cdot 4} = x^{12} \\ (x^4)^6 &= x^{4 \cdot 6} = x^{24} \\ (x^3)^5 &= x^{3 \cdot 5} = x^{15} \\ (3x^2)^4 &= 3^{1 \cdot 4} x^{2 \cdot 4} = 3^4 x^8 = 81x^8 \\ (2x^3)^3 &= 2^{1 \cdot 3} x^{3 \cdot 3} = 2^3 x^9 = 8x^9\end{aligned}$$

$$\begin{aligned}(3x^2)^2(2x^3)^3 &= 3^{1 \cdot 2} x^{2 \cdot 2} 2^{1 \cdot 3} x^3 \cdot 3 \\ &= 3^2 x^4 2^3 x^9 \\ &= 9 \cdot 8x^{4+9} \\ &= 72x^{13}\end{aligned}$$

$$\begin{aligned}(3^2 x^3 y^4)^2 (2^3 x^2 y^5)^3 &= (3^{2 \cdot 2} x^{3 \cdot 2} y^{4 \cdot 2}) (2^{3 \cdot 3} x^{2 \cdot 3} y^{5 \cdot 3}) \\ &= (3^4 x^6 y^8) (2^9 x^6 y^{15}) \\ &= (81 x^6 y^8) (512 x^6 y^{15}) \\ &= 81 \cdot 512 x^6 + 6 y^{8+15} \\ &= 41472 x^{12} y^{23}\end{aligned}$$





$$\begin{aligned}-2^3 &= -2 \cdot -2 \cdot -2 = -8 \\ (-2)^3 &= -2 \cdot -2 \cdot -2 = -8 \\ -(-2)^3 &= -2 \cdot -2 \cdot -2 = 8\end{aligned}$$

$$\begin{aligned}(-7x^2y^3)^0 &= -7^{2 \cdot 0}x^{2 \cdot 0}y^{3 \cdot 0} \\ &= -7^0x^0y^0 \\ &= 1 \cdot 1 \cdot 1 \\ &= 1\end{aligned}$$

$$\begin{aligned}3x(5x + 8) &= 15x^2 + 24x \\ 4x(x^2 - 2x + 3) &= 4x^3 - 8x^2 + 12x\end{aligned}$$





## I Dividing Polynomials

### Fraction Components

- ➔ **Numerator**  $\Rightarrow$  Top of the fraction, counts selected parts, e.g. in  $\frac{3}{4}$  the numerator is 3
- ➔ **Denominator**  $\Rightarrow$  Bottom of the fraction, defines total equal parts, e.g. in  $\frac{3}{4}$  the denominator is 4
- ➔ **Relationship**  $\Rightarrow$  Fraction = Numerator  $\div$  Denominator
- ➔ **Technique**  $\Rightarrow$  Numerator changes with quantity chosen, denominator fixes the partition size
- ➔ **Outcome**  $\Rightarrow$  Understanding both clarifies fraction meaning and operations

$$\frac{x^8}{x^3} = x^{8-3} \Rightarrow x^5 \quad (9)$$

$$\frac{x^5}{x^2} = x^{5-2} \Rightarrow x^3 \quad (10)$$

$$\frac{x^5}{x^8} = x^{5-8} \Rightarrow x^{-3} \quad (11)$$

$$\frac{x^4}{x^7} = x^{4-7} \Rightarrow x^{-3} \quad (12)$$

$$(13)$$





$$\begin{aligned}\frac{24x^9y^5}{8x^3y^{12}} &= \frac{24}{8}x^{9-3}\frac{1}{1}y^{5-12} \\ &= 3x^6y^{-7} \\ &= \frac{3x^6}{y^7}\end{aligned}$$

$$\begin{aligned}\frac{12x^5y^{-3}z^4}{36x^8y^{-4}x^{-8}} &= \frac{\frac{12}{3}x^{5-8}}{\frac{36}{3}}\frac{1}{1}y^{-3-(-4)}\frac{1}{1}z^{4-(-8)} \\ &= \frac{x^{-3}y^1z^{12}}{3} \\ &= \frac{yz^{12}}{3x^3}\end{aligned}$$





## I Multiplying Polynomials

### Multiplication Symbols

- ➔ Dot  $\Rightarrow$   $\cdot$  is clean, algebraic, avoids confusion with  $x$
- ➔ Times  $\Rightarrow$   $\times$  is bold, arithmetic, or cross product
- ➔ Context  $\Rightarrow$  Use  $\cdot$  in algebra,  $\times$  in arithmetic or vectors
- ➔ Technique  $\Rightarrow$  Choose based on clarity and audience
- ➔ Outcome  $\Rightarrow$  Both mean multiplication, but notation signals intent

$$x^2 \cdot x^4 = x^{2+4} \Rightarrow x^6$$

$$x^7 \cdot x^5 = x^{5+7} \Rightarrow x^{12}$$

$$x^8 \cdot x^9 = x^{8+9} \Rightarrow x^{17}$$





$$(3x^3)(5x^6) = (3 \cdot 5)x^{3+6} \Rightarrow 15x^9$$

$$(4x^2)(7x^3) = (4 \cdot 7)x^{2+3} \Rightarrow 28x^5$$

$$(4xy^2)(8x^2y^3) = (4 \cdot 8)x^{1+2}(1 \cdot 1)y^{2+3} \Rightarrow 32x^3y^5$$

$$(5x^2y^3)(6x^3y^4) = (5 \cdot 6)x^{2+3}(1 \cdot 1)y^{3+4} \Rightarrow 30x^5y^7$$

$$(7x^3y^4)(8x^5y^7) = (7 \cdot 8)x^{3+5}(1 \cdot 1)y^{4+7} \Rightarrow 56x^8y^{11}$$





## I Combining Polynomials

$$x + 4 = 7 \Rightarrow x + 4 - 4 = 7 - 4 \Rightarrow x + 0 = 3$$

$$x + 9 = 15 \Rightarrow x + 9 - 9 = 15 - 9 \Rightarrow x + 0 = 6$$

$$6 + x = 13 \Rightarrow 6 + x - 6 = 13 - 6 \Rightarrow 0 + x - 0 = 7$$

$$x - 3 = 9 \Rightarrow x - 3 + 3 = 9 + 3 \Rightarrow x - 0 = 12 \Rightarrow x = 12$$

$$x - 8 = 7 \Rightarrow x + 8 - 8 = 7 + 8 \Rightarrow x - 0 = 15 \Rightarrow x = 15$$

$$3x + 5 = 11 \Rightarrow 3x + 5 - 5 = 11 - 5 \Rightarrow \frac{3x}{3} = \frac{6}{3} \Rightarrow x = 2$$





$$6.3 = -2 + x \Rightarrow 6.3 + 2 = -2 + 2 + x \Rightarrow 6.3 = 0 + x \Rightarrow x = 6.3$$

$$5 = x - 8 \Rightarrow 5 + 8 = x - 8 + 8 \Rightarrow 13 = x - 0 \Rightarrow \\ \hookrightarrow x = 13$$

$$5 - x = 12 \Rightarrow 5 - 12 - x + x = 12 - 12 + x \Rightarrow \\ \hookrightarrow -7 = 0 + x \Rightarrow x = -7$$

$$-8 = 5 - x \Rightarrow -8 + 8 = 5 + 8 - x \Rightarrow 0 + x = 13 - x + x \Rightarrow \\ \hookrightarrow x = 13$$

$$3x = 12 \Rightarrow \frac{3x}{3} = \frac{12}{3} \Rightarrow \frac{x}{1} = 4 \Rightarrow x = 4$$





$$7x = 14 \Rightarrow \frac{7x}{7} = \frac{14}{7} \Rightarrow \frac{x}{1} = 2 \Rightarrow x = 2$$

$$-6x = -30 \Rightarrow \frac{-6x}{-6} = \frac{-30}{-6} \Rightarrow \frac{-x}{-1} = 5 \Rightarrow x = 5$$

$$-8x = 48 \Rightarrow \frac{-8x}{-8} = \frac{48}{-8} \Rightarrow \frac{-x}{-1} = -6 \Rightarrow x = -6$$

$$7x = -56 \Rightarrow \frac{7x}{7} = \frac{-56}{7} \Rightarrow \frac{x}{1} = -8 \Rightarrow x = -8$$

$$-8x = -72 \Rightarrow \frac{-8x}{-8} = \frac{-72}{-8} \Rightarrow \frac{x}{1} = 9 \Rightarrow x = 9$$





$$\begin{aligned}4x + 3 = 6x - 15 &\Rightarrow 4x - 4x + 3 + 15 = 6x - 4x - 15 + 15 \Rightarrow \\&\hookrightarrow \frac{18}{2} = \frac{2x}{2}; \Rightarrow x = 9\end{aligned}$$

$$\begin{aligned}3(2x - 4) = 5(3x + 2) - 3 &\Rightarrow 6x - 12 = 15x + 10 - 3 \Rightarrow \\&\hookrightarrow 6x - 6x - 12 - 7 = 15x - 6x + 7 - 7 \Rightarrow \\&\hookrightarrow \frac{-19}{9} = \frac{9x}{9} \Rightarrow x = \frac{-19}{9}\end{aligned}$$

$$\begin{aligned}\frac{3}{4}x - \frac{2}{3} = 12 &\Rightarrow \left(\frac{3}{4}x \cdot 4\right)3 - \left(\frac{2}{3} \cdot 3\right)4 = 12 \cdot 12 \\&\hookrightarrow (3x)3 - (2)4 = 144 \Rightarrow 9x - 8 + 8 = 144 + 8 \Rightarrow \\&\hookrightarrow \frac{9x}{9} = \frac{152}{9} \Rightarrow x = \frac{152}{9}\end{aligned}$$

$$\begin{aligned}\frac{2}{3}x + 5 = 8 &\Rightarrow \left(\frac{2}{3}x + 5 = 8\right)3 \Rightarrow 2x + 15 - 15 = 24 - 15 \Rightarrow \\&\hookrightarrow \frac{2x}{2} = \frac{9}{2} \Rightarrow x = \frac{9}{2}\end{aligned}$$



$$\begin{aligned}(3x + 5) + (4x - 2) &= 7x + 3 \\(4x^2 + 3x + 9) + (5x^2 + 7x - 4) &= 9x^2 + 10x + 5 \\(5x^2 - 6x - 12) - (7x^2 + 4x - 13) &= 5x^2 - 6x - 12 - 7x^2 - 4x + 13 \\&= 5x^2 - 7x^2 - 12 + 13 - 6x - 4x \\&= -2x^2 + 1 - 10x\end{aligned}$$

## I FOIL Method

$$(a + b)(c + d) = ac + ad + bc + bd \quad (14)$$

**FOIL Method**

- ➔ **First**  $\Rightarrow$  Multiply first terms:  $a \cdot c$
- ➔ **Outer**  $\Rightarrow$  Multiply outer terms:  $a \cdot d$
- ➔ **Inner**  $\Rightarrow$  Multiply inner terms:  $b \cdot c$
- ➔ **Last**  $\Rightarrow$  Multiply last terms:  $b \cdot d$
- ➔ **Outcome**  $\Rightarrow$  Sum all four products to get the expanded expression

$$\begin{aligned}(2x + 5)(4x^2 - 3x + 6) &= (2 \cdot 4)x^{1+2} + (2 \cdot -3)x^{1+1} + (2 \cdot 6)x \\ &\quad \hookrightarrow + (5 \cdot 4)x^2 + (5 \cdot -3)x + (5 \cdot 6) \\ &= 8x^3 + (-6 + 20)x + 30 \\ &= 8x^3 + 14x^2 + -3x + 30\end{aligned}$$



$$\begin{aligned}
 & (3x^2 - 2x + 4)(4x^2 + 5x - 6) = \\
 & \hookrightarrow (3 \cdot 4)x^{2+2} + (3 \cdot 5)x^{2+1} + (3 \cdot -6)x^{2+0} \\
 & \hookrightarrow +(-2 \cdot 4)x^{1+2} + (-2 \cdot 5)x^{1+1} + (-2 \cdot -6)x^{1+0} \\
 & \hookrightarrow +(4 \cdot 4)x^{0+2} + (4 \cdot 5)x^{0+1} + (4 \cdot -6)x^{0+0} \\
 & = 12x^4 + (15 + -8)x^3 + (-18 + -10 + 16)x^2 + (12 + 20)x + -24 \\
 & = 12x^4 + 7x^3 + -12x^2 + 32x + -24
 \end{aligned}$$

## I Factoring Polynomials

$$x + 4 = 7 \Rightarrow x + 4 - 4 = 7 - 4 \Rightarrow x + 0 = 3$$

$$x + 9 = 15 \Rightarrow x + 9 - 9 = 15 - 9 \Rightarrow x + 0 = 6$$

$$6 + x = 13 \Rightarrow 6 + x - 6 = 13 - 6 \Rightarrow 0 + x - 0 = 7$$





$$x - 3 = 9 \Rightarrow x - 3 + 3 = 9 - 3 \Rightarrow x - 0 = 6 \Rightarrow x = 6$$

$$x - 8 = 7 \Rightarrow x + 8 - 8 = 7 + 8 \Rightarrow x - 0 = 15 \Rightarrow x = 15$$

$$3x + 5 = 11 \Rightarrow 3x + 5 - 5 = 11 - 5 \Rightarrow \frac{3x}{3} = \frac{6}{3} \Rightarrow x = 2$$

$$6.3 = -2 + x \Rightarrow 6.3 + 2 = -2 + 2 + x \Rightarrow 6.3 = 0 + x \Rightarrow x = 6.3$$

$$5 = x - 8 \Rightarrow 5 + 8 = x - 8 + 8 \Rightarrow 13 = x - 0 \Rightarrow \\ \hookrightarrow x = 13$$

$$5 - x = 12 \Rightarrow 5 - 12 - x + x = 12 - 12 + x \Rightarrow \\ \hookrightarrow -7 = 0 + x \Rightarrow x = -7$$





$$\begin{aligned} -8 = 5 - x &\Rightarrow -8 + 8 = 5 + 8 - x \Rightarrow 0 + x = 13 - x + x \Rightarrow \\ &\hookrightarrow x = 13 \end{aligned}$$

$$3x = 12 \Rightarrow \frac{3x}{3} = \frac{12}{3} \Rightarrow \frac{x}{1} = 4 \Rightarrow x = 4$$

$$7x = 14 \Rightarrow \frac{7x}{7} = \frac{12}{7} \Rightarrow \frac{x}{1} = 2 \Rightarrow x = 2$$

$$-6x = -30 \Rightarrow \frac{-6x}{-6} = \frac{-30}{-6} \Rightarrow \frac{-x}{-1} = 5 \Rightarrow x = 5$$

$$-8x = 48 \Rightarrow \frac{-8x}{-8} = \frac{48}{-8} \Rightarrow \frac{-x}{-1} = -6 \Rightarrow x = -6$$



$$7x = -56 \Rightarrow \frac{7x}{7} = \frac{-56}{7} \Rightarrow \frac{x}{1} = -8 \Rightarrow x = -8$$

$$-8x = -72 \Rightarrow \frac{-8x}{-8} = \frac{-72}{-8} \Rightarrow \frac{x}{1} = 9 \Rightarrow x = 9$$

$$\begin{aligned} 4x + 3 = 6x - 15 &\Rightarrow 4x - 4x + 3 + 15 = 6x - 4x - 15 + 15 \Rightarrow \\ &\hookrightarrow \frac{18}{2} = \frac{2x}{2}; \Rightarrow x = 9 \end{aligned}$$

$$\begin{aligned} 3(2x - 4) = 5(3x + 2) - 3 &\Rightarrow 6x - 12 = 15x + 10 - 3 \Rightarrow \\ &\hookrightarrow 6x - 6x - 12 - 7 = 15x - 6x + 7 - 7 \Rightarrow \\ &\hookrightarrow \frac{-19}{9} = \frac{9x}{9} \Rightarrow x = \frac{-19}{9} \end{aligned}$$



$$\begin{aligned}\frac{3}{4}x - \frac{2}{3} = 12 &\Rightarrow \left(\frac{3}{4}x \cdot 4\right)3 - \left(\frac{2}{3} \cdot 3\right)4 = 12 \cdot 12 \\ \hookrightarrow (3x)3 - (2)4 = 144 &\Rightarrow 9x - 8 + 8 = 144 + 8 \Rightarrow \\ &\hookrightarrow \frac{9x}{9} = \frac{152}{9} \Rightarrow x = \frac{152}{9}\end{aligned}$$

$$\begin{aligned}\frac{2}{3}x + 5 = 8 &\Rightarrow \left(\frac{2}{3}x + 5 = 8\right)3 \Rightarrow 2x + 15 - 15 = 24 - 15 \Rightarrow \\ &\hookrightarrow \frac{2x}{2} = \frac{9}{2} \Rightarrow x = \frac{9}{2}\end{aligned}$$





## II Glossary

### Glossary

#### Glossary

**Coefficient** The numerical factor that multiplies a variable in a term

**Like Terms** Terms that have the same variable(s) raised to the same power(s)

**Numerator** the top number in a fraction, showing how many parts are taken

**Denominator** The bottom number in a fraction, showing how many equal parts make the whole

**Binomial** A polynomial with two terms. See equation 2.

**Division Rule** Subtract exponents when dividing like bases. Example: see equation 9.